SystemF2Effect: fixing admits in preservation / new
Ignore-this: 1973dcb5eacbf3e52c2dc5dc5ce6ad04

darcs-hash:20130206045436-08f32-d73905c8051581844f7f7f523ccb65f7c9da8aef

devel/Iron/Language/SystemF2Effect/Step/Preservation.v
@@ -1,38 +1,33 @@
 
 Require Export Iron.Language.SystemF2Effect.Step.TfJudge.
 
-Definition WfFS (ss : store) (se : stenv) (fs : stack) (sp : stprops) 
- := Forall closedT se
- /\ STOREP fs sp
- /\ STOREM se ss
- /\ STORET se sp ss.
-
 
 (* When a well typed expression transitions to the next state
    then its type is preserved. *)
 Theorem preservation
- :  forall ss ss' se fs sp fs' x x' t e
- ,  WfFS   ss se fs sp
+ :  forall se sp ss ss' fs fs' x x' t e
+ ,  WfFS   se sp ss fs 
  -> TYPEC  nil nil se fs  x   t  e
  -> STEPF  ss  fs  x  ss' fs' x'
  -> (exists se' sp' e'
             ,  extends se' se
-            /\ WfFS  ss' se' fs' sp'
+            /\ WfFS  se' sp' ss' fs'
             /\ SubsT e e'
             /\ TYPEC nil nil se' fs' x' t e').
 Proof.
- intros ss ss' se fs sp fs' x x' t e HH HC HS. gen sp t e.
+ intros se sp ss ss' fs fs' x x' t e HH HC HS. gen sp t e.
  induction HS; intros; inverts_typec; rip.
 
  (* Pure evaluation. *)
- Case "SfStep".
-  exists se. 
-  exists sp. 
-  exists (TSum e1 e2).
-  rip.
-  eapply TcExp; eauto.
-  eapply stepp_preservation; eauto.
+ Case "SfStep". 
+ { exists se. 
+   exists sp. 
+   exists (TSum e1 e2).
+   rip.
+   eapply TcExp; eauto.
+   eapply stepp_preservation; eauto.
    inverts HH. rip.
+ }
 
  (* Push let context. *)
  Case "SfLetPush".
@@ -44,44 +39,43 @@ Proof.
 
  (* Create a new region. *)
  Case "SfRegionNew".
-  set (r := TCap (TyCapRegion p)).
-  exists se.
-  exists (sp :> SRegion p).
-  exists (TSum (substTT 0 r e) e2).
-  rip.
-   (* Store is well formed under new props. *)
-   admit.   (* ok, WfFs under extended props *)
-
+ { set (r := TCap (TyCapRegion p)).
+   exists se.
+   exists (sp :> SRegion p).
+   exists (TSum (substTT 0 r e) e2).
+   rip.
    admit.   (* NO PRES OF EFFECTS
                We get phase-changed effects for regions in current stack
                because we're inside the use context *)
 
    (* Result is well typed. *)
-   eapply TcExp 
+   + eapply TcExp 
        with (sp := sp0 :> SRegion p) 
-            (t1 := substTT 0 r t0).
-     admit. (* ok, store props model new frame stack *)
-     
-     (* Type is preserved after substituting handle. *)
-     rrwrite (nil = substTE 0 r nil).
-     rrwrite (se  = substTE 0 r se) by admit. (* ok, se is closed *)
-     eapply subst_type_exp with (k2 := KRegion).
-      rrwrite (substTE 0 r nil = nil).
-      rrwrite (substTE 0 r se  = se)  by admit.
-      rrwrite (liftTE 0 nil    = nil).
-      rrwrite (liftTE 0 se     = se)  by admit.
-      admit.  (* ok, weak store props *)
-      subst r. eapply KiCap. 
-       admit. (* ok, lists *)
+            (t1 := substTT 0 r t0); auto.
+
+     (* Type is preserved after substituting region handle. *)
+     - have HTE: (nil = substTE 0 r nil).
+       rewrite HTE.
+
+       have HSE: (se  = substTE 0 r se)
+        by (inverts HH; symmetry; auto).
+       rewrite HSE.
+
+       eapply subst_type_exp with (k2 := KRegion).
+       * rrwrite (liftTE 0 nil    = nil).
+         rrwrite (liftTE 0 se = se) by (inverts HH; auto).
+         auto.
+       * subst r. auto.
 
      (* New frame stack is well typed. *)
-     eapply TfConsUse.
-      admit. (* ok, region handle is fresh, goodness of allocRegionFs *)
-      admit. (* ok, t0 doesn't mention ^0 by lowerTT *)
-  
+     - eapply TfConsUse.
+       admit.                  (* ok, region handle is fresh, goodness of allocRegionFs *)
+       admit.                  (* ok, t0 doesn't mention ^0 by lowerTT *)
+ }
+
  (* Pop a region from ths stack. *)
  Case "SfRegionPop".
-  destruct sp.
+ { destruct sp.
    false. admit.
    destruct s.
     have (n = p) by admit. subst. (* ok from WfSS *)
@@ -99,16 +93,18 @@ Proof.
 
    rrwrite (e2 = TSum (TBot KEffect) e2) by admit.
    eapply TcExp with (t1 := t1).
-    have (STOREP fs sp0) by admit. (* ok, from WfSS *)
+    have (STOREP sp0 fs) by admit. (* ok, from WfSS *)
     eauto.
     eapply TxVal.
      admit. (* ok, get p notin t1 from TYPEF, maybe add premise to TYPEF *)
      rrwrite (TSum (TBot KEffect) e2 = e2) by admit.
       auto.
+ }
 
  (* Allocate a reference. *)
  Case "SfStoreAlloc".
   admit.
+ 
 
  (* Read from a reference. *)
  Case "SfStoreRead".
