devel/Iron/Language/SystemF2Effect/Step/TfJudge.v
@@ -1,12 +1,7 @@
 
 Require Export Iron.Language.SystemF2Effect.Value.TyJudge.
 Require Export Iron.Language.SystemF2Effect.Step.Frame.
-
-
-(* Store properties model use frames on stack. *)
-Definition STOREP (fs : stack) (sp : stprops)
- := forall n, In (FUse n) fs <-> In (SRegion n) sp.
-
+Require Export Iron.Language.SystemF2Effect.Store.
 
 (* Type of a frame stack.
    The frame stack is like a continuation that takes an expression of a certain
@@ -18,7 +13,7 @@ Inductive TYPEF : kienv -> tyenv -> stenv -> stack -> ty -> ty -> ty -> Prop :=
 
  | TfConsLet
    :  forall ke te se fs sp t1 x2 t2 e2 t3 e3
-   ,  STOREP fs sp
+   ,  STOREP sp fs
    -> TYPEX  ke (te :> t1) se sp                 x2 t2 e2
    -> TYPEF  ke te         se fs                 t2 t3 e3
    -> TYPEF  ke te         se (fs :> FLet t1 x2) t1 t3 (TSum e2 e3)
@@ -46,12 +41,12 @@ Ltac inverts_typef :=
 Inductive TYPEC : kienv -> tyenv -> stenv -> stack -> exp -> ty -> ty -> Prop :=
  | TcExp
    :  forall ke te se sp fs x1 t1 e1 t2 e2
-   ,  STOREP fs sp
+   ,  STOREP sp fs
    -> TYPEX  ke te se sp x1 t1 e1
    -> TYPEF  ke te se fs t1 t2 e2
    -> TYPEC  ke te se fs x1 t2 (TSum e1 e2).
 Hint Constructors TYPEC.
-(* TODO: going to need to mask effects involving region handles from e1 *)
+
 
 Ltac inverts_typec :=
  repeat
