devel/Iron/Language/SystemF2Effect/Step/Pure.v
@@ -1,7 +1,7 @@
 
-Require Export Iron.Language.SystemF2Effect.Store.
 Require Export Iron.Language.SystemF2Effect.Type.
 Require Export Iron.Language.SystemF2Effect.Value.
+Require Export Iron.Language.SystemF2Effect.Store.Bind.
 
 
 (* Small Step Evaluation (pure rules)
