devel/Iron/Language/SystemF2Effect/Type/KiJudge.v
@@ -224,5 +224,21 @@ Proof.
   eapply KiCon2.
   destruct t1. simpl in *. eauto.
   eauto. eauto.
-Qed.  
+Qed.
+
+
+Lemma kind_stprops_cons
+ :  forall ke sp p t k
+ ,  KIND ke sp t k
+ -> KIND ke (sp :> p) t k.
+Proof.
+ intros. gen ke k.
+ induction t; intros; inverts_kind; burn.
   
+ Case "TCon2".
+  destruct tc. snorm. inverts H2.
+  eapply KiCon2; eauto.
+  destruct t1. snorm.
+Qed.
+
+
